hygiene_help.v
@@ -3,10 +3,10 @@ From Coq Require Import ssreflect ssrfun ssrbool.
 From mathcomp Require Import seq eqtype ssrnat.
 From istari Require Import lemmas0
      source subst_src rules_src basic_types
-     help subst_help0 subst_help trans derived_rules embedded_lemmas proofs.
+     help subst_help0 subst_help.
 From istari Require Import Sigma Tactics
      Syntax Subst SimpSub Promote Hygiene
-     ContextHygiene Equivalence Equivalences Rules Defined.
+     ContextHygiene Equivalence Equivalences Rules Defined DefsEquiv.
 
 Definition hctx G := @hygiene False (@ctxpred False G).
 
@@ -195,7 +195,7 @@ Hint Resolve hygiene_pi hygiene_karrow hygiene_arrow hygiene_lam hygiene_app
      hygiene_bfalse hygiene_btrue hygiene_bite hygiene_prod hygiene_sigma hygiene_ppair
      hygiene_ppi1 hygiene_ppi2 hygiene_wt hygiene0 hygiene_hint hygiene2 hygiene3 hygiene_univ: hygiene_hint.
 
-Ltac hyg_solv := eauto 50 with hygiene_hint.
+Ltac hyg_solv := try (prove_the_hygiene; simpl; auto); eauto 50 with hygiene_hint.
 
 Lemma hygiene_makesubseq G: (hctx G) make_subseq.
 unfold make_subseq. hyg_solv. Qed.
@@ -210,7 +210,7 @@ Lemma hygiene_moveapp G A m v: (hctx G) m ->
 Qed.
 
 Lemma hygiene_nat G: (hctx G) nattp.
-  intros. unfold nattp. hyg_solv. Qed.
+  prove_the_hygiene. simpl. auto. Qed.
 
 Lemma hygiene_nzero: forall G, (hctx G) nzero.
    unfold nzero. hyg_solv. Qed.
@@ -235,104 +235,86 @@ Lemma hygiene_minus G : (hctx G) minus.
   unfold minus. unfold minusbc. hyg_solv. Qed.
 Hint Resolve hygiene_minus: hygiene_hint.
 
+Lemma hygiene_sh1 G n x: (hctx G) n ->
+                         hctx (x :: G) (subst sh1 n).
+  intros. eapply hygiene_shift'.
+  rewrite ctxpred_length.
+  match goal with |- hygiene ?f ?n => suffices: hincl (ctxpred G) f end. 
+  move => Hincl. apply (hygiene_weaken _ _ _ _ Hincl).
+  assumption. rewrite ctxpred_length. move =>> Hi. simpl.
+  omega. Qed.
+
+
+Lemma hygiene_sh3 G n x y z: (hctx G) n ->
+                         hctx (x :: y:: z::G) (subst (sh 3) n).
+  intros. eapply hygiene_shift'.
+  rewrite ctxpred_length.
+  match goal with |- hygiene ?f ?n => suffices: hincl (ctxpred G) f end. 
+  move => Hincl. apply (hygiene_weaken _ _ _ _ Hincl).
+  assumption. rewrite ctxpred_length. move =>> Hi. simpl.
+  omega. Qed.
+
+Lemma hygiene_sh2 G n x y: (hctx G) n ->
+                         hctx (x :: y:: G) (subst (sh 2) n).
+  intros. eapply hygiene_shift'.
+  rewrite ctxpred_length.
+  match goal with |- hygiene ?f ?n => suffices: hincl (ctxpred G) f end. 
+  move => Hincl. apply (hygiene_weaken _ _ _ _ Hincl).
+  assumption. rewrite ctxpred_length. move =>> Hi. simpl.
+  omega. Qed.
+
+Lemma hygiene_sh4 G n x y z a: (hctx G) n ->
+                         hctx (x :: y:: z:: a :: G) (subst (sh 4) n).
+  intros. eapply hygiene_shift'.
+  rewrite ctxpred_length.
+  match goal with |- hygiene ?f ?n => suffices: hincl (ctxpred G) f end. 
+  move => Hincl. apply (hygiene_weaken _ _ _ _ Hincl).
+  assumption. rewrite ctxpred_length. move =>> Hi. simpl.
+  omega. Qed.
+
+Hint Resolve hygiene_sh1 hygiene_sh2 hygiene_sh3 hygiene_sh4: hygiene_hint.
+
 Lemma hygiene_nsucc G n: (hctx G) n -> (hctx G) (nsucc n).
   intros. unfold nsucc. hyg_solv. Qed.
+
+Hint Resolve hygiene_nsucc: hygiene_hint.
 
 Lemma hygiene_ltb G : (hctx G) lt_b.
   intros. unfold lt_b. unfold if_z. hyg_solv. Qed.
 Hint Resolve hygiene_ltb: hygiene_hint.
 
 Lemma hygiene_world: forall G, (hctx G) world.
-intros. unfold world. unfold preworld. unfold nattp. auto. Qed.  
+intros. unfold world. hyg_solv. Qed.  
 Hint Resolve hygiene_world: hygiene_hint.
 
 
-Hint Resolve hygiene_nat: hygiene_hint.
+Lemma hygiene_leqtp: forall G, (hctx G) leqtp.
+  intros. hyg_solv. Qed. 
+
+Lemma hygiene_bind: forall G m1 m2, (hctx G) m1 -> (hctx G) m2 ->
+                               (hctx G) (make_bind m1 m2).
+  intros. hyg_solv. Qed.
 
 
-Lemma hygiene_leqtp: forall G, (hctx G) leqtp
-  intros. unfold leqtp. unfold wind. unfold theta.
-  repeat rewrite hygiene_app.
-  repeat rewrite hygiene_lam. hyg_solv. simpl.
-  repeat rewrite project_dot_succ.
-  rewrite project_dot_zero. auto. Qed.
-Hint Resolve hygiene_leqtp: hygiene_hint.
+Lemma hygiene_lttp: forall G, (hctx G) lttp.
+  intros. hyg_solv. Qed.
 
-Lemma hygiene_bind: forall G, (hctx G) make_bind (@hygiene False s m1) (@hygiene False s m2)
-  intros. auto. Qed.
-
-
-Lemma hygiene_lttp: forall G, (hctx G) lttp
-  intros. unfold lttp.
-  hyg_solv. rewrite hygiene_leqtp. unfold nsucc. hyg_solv. simpl.
-  rewrite hygiene_leqtp. auto. Qed.
-Hint Resolve hygiene_leqtp: hygiene_hint.
-
-Lemma hygiene_leq: forall s n1 n2,
-    @hygiene False s (leq_t n1 n2) =  leq_t (hygiene s n1) (hygiene s n2).
-  intros. unfold leq_t.  repeat rewrite hygiene_app. auto. 
+Lemma hygiene_leq: forall G m1 m2, (hctx G) m1 -> (hctx G) m2 ->
+                               (hctx G) (leq_t m1 m2).
+  intros. hyg_solv. 
 Qed.
+Hint Resolve hygiene_bind hygiene_leqtp hygiene_lttp: hygiene_hint.
 
-Lemma hygiene_lt: forall s n1 n2,
-    hygiene s (lt_t n1 n2) = lt_t (hygiene s n1) (@hygiene False s n2).
-  intros. repeat rewrite hygiene_app. rewrite hygiene_lttp. auto. Qed. 
+Lemma hygiene_subseq: forall G m1 m2, (hctx G) m1 -> (hctx G) m2 ->
+                                 (hctx G) (subseq m1 m2).
+  intros. unfold subseq. hyg_solv. Qed.
 
-Lemma hygiene_subseq: forall W1 W2 s,
-       (hygiene s
-              (subseq W1 W2)) = subseq (hygiene s W1)
-                                       (hygiene s W2).
-  intros. unfold subseq. repeat rewrite hygiene_app. auto.
-Qed.
+Hint Resolve hygiene_subseq: hygiene_hint.
 
-
-
-Lemma hygiene_ret: forall G, (hctx G) ret
-  intros. unfold ret. unfold inl. hyg_solv. Qed.
-
-Lemma hygiene_ret_a: forall s m, hygiene s (ret_a m) = ret_a (hygiene s m).
-  intros. unfold ret_a. unfold ret. unfold inl. hyg_solv. Qed.
-
-Lemma hygiene_laters: forall s A, (hygiene s (laters A)) = (laters (hygiene s A)).
-  intros. unfold laters. unfold plus. rewrite hygiene_rec. rewrite hygiene_sigma.
-  rewrite hygiene_booltp. rewrite hygiene_bite. hyg_solv. simpl.
-  repeat rewrite <- hygiene_sh_shift. hyg_solv. Qed.
-
-Lemma hygiene_nth: forall s m1 m2, (hygiene s (nth m1 m2)) = (nth (hygiene s m1) (hygiene s m2)). intros. unfold nth. hyg_solv. Qed.
-
-Lemma hygiene_make_subseq: forall s, (hygiene s make_subseq) = make_subseq.
-  intros. unfold make_subseq. hyg_solv. Qed.
-
-Lemma hygiene_picomp1: forall s m, (hygiene s (picomp1 m)) = picomp1 (hygiene s m).
-  intros. unfold picomp1. hyg_solv. Qed.
-
-Lemma hygiene_picomp2: forall s m, (hygiene s (picomp2 m)) = picomp2 (hygiene s m).
-  intros. unfold picomp2. hyg_solv. Qed.
-
-Lemma hygiene_picomp3: forall s m, (hygiene s (picomp3 m)) = picomp3 (hygiene s m).
-  intros. unfold picomp3. hyg_solv. Qed.
-
-Lemma hygiene_picomp4: forall s m, (hygiene s (picomp4 m)) = picomp4 (hygiene s m).
-  intros. unfold picomp4. hyg_solv. Qed.
-
-Hint Resolve hygiene_U0 hygiene_ret hygiene_ret_a hygiene_subseq hygiene_leq hygiene_leq
-     hygiene_lttp hygiene_lt hygiene_nzero hygiene_nat hygiene_world hygiene_pw hygiene_world
-     hygiene_nth hygiene_laters hygiene_picomp1 hygiene_picomp2 hygiene_picomp4
-     hygiene_picomp3 hygiene_make_subseq hygiene_theta hygiene_minus hygiene_ltb: hygiene_hint.
-
-Hint Resolve <- hygiene_sh_shift: hygiene_hint.
-
-Hint Unfold hygiene_hint: hygiene_hint.
-
-
-Lemma hygiene_store: forall w l s, hygiene s (store w l) = store (hygiene s w) (hygiene s l).
-  intros. unfold store. unfold gettype. hyg_solv_big. auto. Qed.
+Lemma hygiene_store: forall G m1 m2, (hctx G) m1 -> (hctx G) m2 ->
+                               (hctx G) (store m1 m2).
+  intros. unfold store. unfold gettype.
+  rewrite - ! subst_sh_shift. hyg_solv. Qed.
 
 Hint Resolve hygiene_store: hygiene_hint.
 
-
-
-Lemma hygiene_moveapp s A m1 m2 : (hygiene s (move_app A m1 m2)) =
-                              move_app A (hygiene s m1) (hygiene s m2).
-   unfold move_app. hyg_solv_big. auto. Qed.
-
-Hint Resolve hygiene_nsucc hygiene_moveapp: hygiene_hint.
